LeanSts/Tactics.lean
@@ -22,13 +22,59 @@ def fresh [Monad m] [Lean.MonadLCtx m] (suggestion : Lean.Name) : m Lean.Syntax.
 def isPrimed (n : Name) : Bool := n.getString!.endsWith "'"
 def getNumPrimes (n : Name) : Nat := n.getString!.foldl (fun n c => if c == '\'' then n + 1 else n) 0
 
+/-- Is `hyp` an application of `n`, after normalisation? -/
+def normalisedIsAppOf (hyp : LocalDecl) (n : Name) : TacticM Bool := do
+  let norm ← Meta.reduce (hyp.type) (skipTypes := false)
+  return norm.isAppOf n
+
+/-- Returns the hypotheses in `newCtx` that do not appear in `oldCtx`. -/
+def newHypotheses (oldCtx : LocalContext) (newCtx : LocalContext) : TacticM (Array LocalDecl) := do
+  let mut newHyps := #[]
+  for hyp in newCtx do
+    if (oldCtx.findFromUserName? hyp.userName |>.isNone) &&
+       !hyp.isImplementationDetail then
+      newHyps := newHyps.push hyp
+  return newHyps
+
+/-- Run the given tactic in all goals. -/
+def allGoals [Inhabited α]
+  (tac : TacticM α) (comb : List α -> α := fun _ => default)  : TacticM α := do
+  if (<- getUnsolvedGoals).length == 0 then
+    tac
+  else
+    withMainContext do
+      let mvarIds ← getUnsolvedGoals
+      let mut mvarIdsNew := #[]
+      let mut ans := []
+      for mvarId in mvarIds do
+        unless (← mvarId.isAssigned) do
+          setGoals [mvarId]
+          let (ans', mvarIdsNew') <- withMainContext do
+            let mut ans := ans
+            let mut mvarIdsNew := mvarIdsNew
+            try
+              let a <- tac
+              ans := a :: ans
+              mvarIdsNew := mvarIdsNew ++ (← getUnsolvedGoals)
+            catch ex =>
+              if (← read).recover then
+                -- logException ex
+                mvarIdsNew := mvarIdsNew.push mvarId
+              else
+                throw ex
+            return (ans, mvarIdsNew)
+          (ans, mvarIdsNew) := (ans', mvarIdsNew')
+      setGoals mvarIdsNew.toList
+      return comb ans
+
+
 /-- Destruct a structure into its fields.
     If no identifier is provided, destructs the goal. -/
 elab "sdestruct " ids:(colGt ident)* : tactic => withMainContext do
   if ids.size == 0 then
     evalTactic $ ← `(tactic| repeat' constructor)
   else for id in ids do
-    let lctx ← Lean.MonadLCtx.getLCtx
+    let lctx ← getLCtx
     let name := (getNameOfIdent' id)
     let .some ld := lctx.findFromUserName? name
       | throwError "sdestruct: {id} is not in the local context"
@@ -43,10 +89,10 @@ elab "sdestruct " ids:(colGt ident)* : tactic => withMainContext do
 elab "sintro " ids:(colGt ident)* : tactic => withMainContext do
   evalTactic $ ← `(tactic| intro $(ids)* ; sdestruct $(ids)*)
 
+
 elab "sts_induction" : tactic => withMainContext do
-  let lctx ← Lean.MonadLCtx.getLCtx
   -- (1) Identify the `next` hypothesis
-  let opt_hnext ← lctx.findDeclM? fun (ldecl : Lean.LocalDecl) => do
+  let opt_hnext ← (← getLCtx).findDeclM? fun (ldecl : Lean.LocalDecl) => do
     let declExpr := ldecl.toExpr
     let declType ← Meta.inferType declExpr
     if declType.isAppOf `RelationalTransitionSystem.next then
@@ -57,12 +103,31 @@ elab "sts_induction" : tactic => withMainContext do
   | none => throwError "sts_induction tactic failed: no `next` hypothesis found"
   | some hnext => pure hnext
   let hnextName := mkIdent hnext.userName
-  let htrName ← fresh "htr"
-  evalTactic  $ ← `(tactic| revert $hnextName; intro $htrName:ident)
-  let case_split ← `(tactic| repeat' (rcases $htrName:ident with $htrName | $htrName))
+  -- Create as many goals as `hnext` has constructors.
+  -- For CIC-style systems, `.next` has the form `∃ (_t: [TransitionType]) True`,
+  -- so we first destruct the existential quantifier.
+  if ← normalisedIsAppOf hnext `Exists then
+    evalTactic $ ←  `(tactic| rcases $hnextName:ident with ⟨$hnextName, _⟩)
+  -- NOTE: context has changed, so we need this again
+  withMainContext do
   -- (2) Destruct the `next` hypothesis into separate goals for each individual action
-  evalTactic $ case_split
-  return
+  -- We have two possibilities. Either:
+  -- (a) `next` is a sequence of `∨`'ed propositions
+  -- (b) `next` is an inductive type, in which case we can use `cases` to destruct it.
+  if ← normalisedIsAppOf hnext `Or then
+    -- FIXME: make sure we only break `Or`s, not other things
+    let case_split ← `(tactic| repeat' (rcases $hnextName:ident with $hnextName | $hnextName))
+    evalTactic case_split
+  else -- TODO: check that this is an inductive type
+    -- Inspired by `scase` in LeanSSR: https://github.com/verse-lab/lean-ssr/blob/29ba85c915de17602ba224558e6ebaf2a2845786/Ssreflect/Elim.lean#L11
+    let oldHyps ← getLCtx
+    evalTactic $ ← `(tactic| unhygienic cases $hnextName:ident)
+    withMainContext $ allGoals $ do
+    let newHyps ← newHypotheses oldHyps (← getLCtx)
+    -- dbg_trace "newHyps: {newHyps.map (·.userName)}"
+    assert! newHyps.size == 1
+    let newHypName := mkIdent newHyps[0]!.userName
+    evalTactic $ ← `(tactic| revert $newHypName:ident; intro $hnextName:ident)
 
 /--
   `exact_state` is usually used after `funcases` ar `funcasesM`. At this point the goal should
